Prove sim_configuration_certify_all

src/localdrf/LocalDRFDef.v
@@ -31,26 +31,19 @@ Set Implicit Arguments.
 
 
 
-Inductive step_all A B C D (step: A -> B -> C -> D -> Prop): C -> D -> Prop :=
-| step_all_intro
-    a b c d
-    (STEP: step a b c d)
-  :
-    step_all step c d.
-
 Section LOCALDRF.
 
   Variable L: Loc.t -> bool.
 
-  Definition valid_event (e: ThreadEvent.t): Prop :=
+  Definition pf_event (e: ThreadEvent.t): Prop :=
     forall loc from to msg kind (PROMISE: e = ThreadEvent.promise loc from to msg kind) (LOC: L loc),
       msg = Message.reserve.
 
-  Definition valid_step (e: MachineEvent.t) (tid: Ident.t)
+  Definition pf_step (e: MachineEvent.t) (tid: Ident.t)
              (c0 c1: Configuration.t): Prop :=
     exists lang tr,
       (<<STEP: @Trace.configuration_step lang tr e tid c0 c1>>) /\
-      (<<VALID: List.Forall (compose valid_event snd) tr>>).
+      (<<PF: List.Forall (compose pf_event snd) tr>>).
 
   Inductive configuration_steps_trace:
     forall (c0 c1: Configuration.t) (tr: list (Ident.t * sigT Trace.t)), Prop :=
@@ -61,24 +54,53 @@ Section LOCALDRF.
   | configuration_steps_trace_cons
       c0 c1 c2 trs lang tr e tid
       (STEPS: configuration_steps_trace c0 c1 trs)
-      (STEP: @Trace.configuration_step lang tr e tid c0 c1)
-      (VALID: List.Forall (compose valid_event snd) tr)
+      (STEP: @Trace.configuration_step lang tr e tid c1 c2)
+      (PF: List.Forall (compose pf_event snd) tr)
     :
-      configuration_steps_trace c0 c2 (trs ++ [(tid, existT _ _ tr)]) (* add at "last" *)
+      configuration_steps_trace c0 c2 (trs ++ [(tid, existT _ _ tr)])
   .
+
+  Lemma configuration_steps_trace_1n c0 c1 c2 lang tr trs e tid
+        (STEPS: configuration_steps_trace c1 c2 trs)
+        (STEP: @Trace.configuration_step lang tr e tid c0 c1)
+        (PF: List.Forall (compose pf_event snd) tr)
+    :
+      configuration_steps_trace c0 c2 ((tid, existT _ _ tr)::trs).
+  Proof.
+    ginduction STEPS.
+    { i. eapply configuration_steps_trace_cons with (trs:=[]); eauto. econs. }
+    { i. exploit IHSTEPS; eauto. i. erewrite List.app_comm_cons. econs; eauto. }
+  Qed.
+
+  Lemma configuration_steps_trace_trans c0 c1 c2 trs0 trs1
+        (STEPS0: configuration_steps_trace c0 c1 trs0)
+        (STEPS1: configuration_steps_trace c1 c2 trs1)
+    :
+      configuration_steps_trace c0 c2 (trs0 ++ trs1).
+  Proof.
+    ginduction STEPS1.
+    { i. erewrite List.app_nil_r. eauto. }
+    { i. exploit IHSTEPS1; eauto. i. erewrite List.app_assoc. econs; eauto. }
+  Qed.
 
   Inductive racy_read (loc: Loc.t) (ts: Time.t):
     forall lang (th: Thread.t lang) (e: ThreadEvent.t), Prop :=
   | racy_read_read
       lang (th: Thread.t lang)
       valr releasedr ordr
-      (VIEW: Time.lt (th.(Thread.local).(Local.tview).(TView.cur).(View.rlx) loc) ts)
+      (VIEW:
+         if Ordering.le Ordering.relaxed ordr
+         then Time.lt (th.(Thread.local).(Local.tview).(TView.cur).(View.rlx) loc) ts
+         else Time.lt (th.(Thread.local).(Local.tview).(TView.cur).(View.pln) loc) ts)
     :
       racy_read loc ts th (ThreadEvent.read loc ts valr releasedr ordr)
   | racy_read_update
       lang (th: Thread.t lang)
       to valr valw releasedr releasedw ordr ordw
-      (VIEW: Time.lt (th.(Thread.local).(Local.tview).(TView.cur).(View.rlx) loc) ts)
+      (VIEW:
+         if Ordering.le Ordering.relaxed ordr
+         then Time.lt (th.(Thread.local).(Local.tview).(TView.cur).(View.rlx) loc) ts
+         else Time.lt (th.(Thread.local).(Local.tview).(TView.cur).(View.pln) loc) ts)
     :
       racy_read loc ts th (ThreadEvent.update loc ts to valr valw releasedr releasedw ordr ordw)
   .
@@ -99,8 +121,8 @@ Section LOCALDRF.
       racy_write loc ts th (ThreadEvent.update loc from ts valr valw releasedr releasedw ordr ordw)
   .
 
-  Definition racefree (s: Threads.syntax): Prop :=
-    forall c0 c1 trs
+  Definition racefree (c0: Configuration.t): Prop :=
+    forall c1 trs
            loc ts
            tid0 tid1 lang0 lang1 tr0 tr1 th0 th1 e0 e1
            (CSTEPS: configuration_steps_trace c0 c1 trs)
@@ -112,11 +134,68 @@ Section LOCALDRF.
            (READ: racy_read loc ts th1 e1),
       False.
 
+  Lemma step_racefree c0 c1 lang tr e tid
+        (RACEFREE: racefree c0)
+        (STEP: @Trace.configuration_step lang tr e tid c0 c1)
+        (PF: List.Forall (compose pf_event snd) tr)
+    :
+      racefree c1.
+  Proof.
+    ii. eapply RACEFREE.
+    { eapply configuration_steps_trace_1n; eauto. }
+    { ss. right.  eapply TRACE0. }
+    { ss. right.  eapply TRACE1. }
+    { eauto. }
+    { eauto. }
+    { eauto. }
+    { eauto. }
+  Qed.
+
+  Lemma steps_racefree c0 c1 trs
+        (RACEFREE: racefree c0)
+        (STEP: configuration_steps_trace c0 c1 trs)
+    :
+      racefree c1.
+  Proof.
+    ii. eapply RACEFREE.
+    { eapply configuration_steps_trace_trans; eauto. }
+    { eapply List.in_or_app. right. eapply TRACE0. }
+    { eapply List.in_or_app. right. eapply TRACE1. }
+    { eauto. }
+    { eauto. }
+    { eauto. }
+    { eauto. }
+  Qed.
+
+  Lemma racefree_write_read c0 c1 c2 trs0 trs1
+        loc ts tid0 tid1 lang0 lang1 tr0 tr1 th0 th1 e0 e1
+        (RACEFREE: racefree c0)
+        (STEPS0: configuration_steps_trace c0 c1 trs0)
+        (STEPS1: configuration_steps_trace c1 c2 trs1)
+        (TRACE0: List.In (tid0, existT _ lang0 tr0) trs0)
+        (TRACE1: List.In (tid1, existT _ lang1 tr1) trs1)
+        (EVENT0: List.In (th0, e0) tr0)
+        (EVENT1: List.In (th1, e1) tr1)
+        (WRITE: racy_write loc ts th0 e0)
+        (READ: racy_read loc ts th1 e1)
+    :
+      False.
+  Proof.
+    eapply RACEFREE.
+    { eapply configuration_steps_trace_trans; eauto. }
+    { eapply List.in_or_app. left. eapply TRACE0. }
+    { eapply List.in_or_app. right. eapply TRACE1. }
+    { eauto. }
+    { eauto. }
+    { eauto. }
+    { eauto. }
+  Qed.
+
   Theorem local_DRF_PF s
-          (RACEFRFEE: racefree s)
+          (RACEFRFEE: racefree (Configuration.init s))
     :
       behaviors Configuration.step (Configuration.init s) <1=
-      behaviors valid_step (Configuration.init s).
+      behaviors pf_step (Configuration.init s).
   Admitted.
 
 End LOCALDRF.
